caseStudy/ADT/costAware/Cost2List.dfy
@@ -3,24 +3,51 @@ include "../../../theory/math/TypeR0.dfy"
 include "../../../theory/ComplexityR0.dfy"
 include "../../../theory/math/TypeR0.dfy"
 include "../Container.dfy"
+include "./Cost2.dfy"
 
 /******************************************************************************
   List ADT
   An indexed collection of elements
 ******************************************************************************/
 
-module List {
+module Cost2List {
 
   import opened TypeR0
   import opened ExpReal
   import opened ComplexityR0
   import opened Container
+  import opened Cost2
 
-  trait List<T> extends Container<T> {
+  trait Cost2List<T, OpType, State> {
 
     /******************************************************************************
       Query operations
     ******************************************************************************/
+
+    // Returns the size of the container
+    function Size(): nat
+      reads this, Repr()
+      // Pre:
+      requires Valid()
+
+    // Returns the element at position i in the container
+    function Get(i:nat): (T, ghost R0)
+      reads this, Repr()
+      // Pre:
+      requires Valid()
+      requires 0 <= i < Size()
+
+    // Returns the set of heap objects that are part of this data structure's representation
+    function Repr(): set<object>
+      reads this
+
+    // Returns true iff the data structure's invariant holds
+    ghost predicate Valid()
+      reads this, Repr()   
+
+    ghost predicate ValidModel()
+      reads this, Repr()  
+      requires Valid()       
 
     // Returns the capacity of the list
     function Capacity(): nat
@@ -42,42 +69,30 @@ module List {
     ******************************************************************************/
 
     // Inserts element x at position k in the list
-    method Insert(k:nat, x:T) returns (ghost t:R0)
+    method Insert(k:nat, x:T) returns (ghost c:Cost2<OpType, State>)
       modifies this, Repr()    
       // Pre:
-      requires Valid()
+      requires Valid() && ValidModel()
       requires 0 <= k <= Size()
       requires !IsFull()
       // Post:
-      ensures  Valid()
+      ensures  Valid() && ValidModel()
       ensures  Size() == old(Size()) + 1
       ensures  forall j :: 0 <= j < k           ==> Get(j).0 == old(Get(j).0)    // [0, k)           is unchanged  
       ensures  forall j :: k < j <= old(Size()) ==> Get(j).0 == old(Get(j-1).0)  // [k, old(Size())) is right shifted  
       ensures  Get(k).0 == x                                                     // xs[k] == x
 
     // Appends element x in the list
-    method Append(x:T) returns (ghost t:R0)
+    method Append(x:T) returns (ghost c:Cost2<OpType, State>)
       modifies this, Repr()    
       // Pre:
-      requires Valid()
+      requires Valid() && ValidModel()
       requires !IsFull()
       // Post:
-      ensures  Valid()
+      ensures  Valid() && ValidModel()
       ensures  Size() == old(Size()) + 1
       ensures  forall j :: 0 <= j < old(Size()) ==> Get(j).0 == old(Get(j).0)    // [0, old(Size())) is unchanged  
       ensures  Get(old(Size())).0 == x                                    
-
-    // Deletes element at position k in the list
-    method Delete(k:nat) returns (ghost t:R0)
-      modifies this, Repr()    
-      // Pre:
-      requires Valid()
-      requires 0 <= k < Size()
-      // Post:
-      ensures  Valid()
-      ensures  Size() == old(Size()) - 1
-      ensures  forall j :: 0 <= j < k      ==> Get(j).0 == old(Get(j).0)
-      ensures  forall j :: k <= j < Size() ==> Get(j).0 == old(Get(j+1).0)
 
   }  
 
