caseStudy/ADT/costAware/CostArrayList.dfy
@@ -1,24 +1,24 @@
-include "../../../../theory/math/ExpReal.dfy"
-include "../../../../theory/math/TypeR0.dfy"
-include "../../../../theory/ComplexityR0.dfy"
-include "../List.dfy"
-include "./LemArrayList.dfy"
+include "../../../theory/math/ExpReal.dfy"
+include "../../../theory/math/TypeR0.dfy"
+include "../../../theory/ComplexityR0.dfy"
+include "./CostList.dfy"
+//include "./LemArrayList.dfy"
 //include "./CostArrayList.dfy"
 
 /******************************************************************************
   Array implementation of a List
 ******************************************************************************/
 
-module ArrayList refines List {
+module CostArrayList refines CostList {
 
-  import opened LemArrayList
+  //import opened LemArrayList
   
   // Refine input type for each relevant operation
   type InsertIn<T> = (array<T>, nat, nat, T)    
   type AppendIn<T> = (array<T>, nat, T)   
   type OkIn<T> = (array<T>, nat)   
 
-  class ArrayList<T(0)> extends List<T> {
+  class ArrayList<T(0)> extends CostList<T> {
 
     var arr:array<T>
     var nElems:nat
@@ -73,10 +73,10 @@ module ArrayList refines List {
       requires Valid()
       requires 0 <= i < Size() 
       // Complexity:
-      ensures var t := ret.1; t <= Tget(Size())
-      ensures var t := ret.1; tIsBigO(Size(), t as R0, constGrowth())      
+      //ensures var t := ret.1; t <= Tget(Size())
+      //ensures var t := ret.1; tIsBigO(Size(), t as R0, constGrowth())      
     {
-      lem_Get_TgetBigOconst();
+      //lem_Get_TgetBigOconst();
       (arr[i], ghost 1.0)
     }
 
@@ -103,9 +103,11 @@ module ArrayList refines List {
     /******************************************************************************
       Update operations
     ******************************************************************************/
+    
+    //Experiment with cost objects
 
     // Inserts element x at position k in the list
-    method Insert(k:nat, x:T) returns (ghost t:R0)
+    method Insert_CostTest(k:nat, x:T) returns (ghost c:Cost<InsertIn<T>>)
       modifies this, Repr()    
       // Pre:
       requires Valid()
@@ -118,11 +120,10 @@ module ArrayList refines List {
       ensures  forall j :: k < j <= old(Size()) ==> Get(j).0 == old(Get(j-1).0)  // [k, old(Size())) is right shifted 
       ensures  Get(k).0 == x                                                     // xs[k] == x
       // Complexity:
-      ensures  var N := old(Size()); && t == Tinsert(N,k)
-                                     && tIsBigO(N, t as R0, linGrowth())                             
-    {
-      var N := Size();
-      t := 0.0;
+      ensures  var N := old(Size()); c.Count() == InsertCost<T>.Cost(N, k)
+    { 
+      c := new InsertCost(arr, nElems, k, x); 
+      var N := Size(); // == nElems
 
       // Update model
       elems := elems[..k] + [x] + elems[k..];
@@ -130,34 +131,31 @@ module ArrayList refines List {
       // Update array:
       // 1. Shift [k, N) to the right
       for i := N downto k
-        modifies arr
+        modifies arr, c
         invariant N < arr.Length
         invariant arr[..i]      == old(arr[..i])   // [0, i) is unchanged  
         invariant arr[i+1..N+1] == old(arr[i..N])  // (i, N) is right shifted        
-        invariant t == (N - i) as R0    
+        invariant c.Count() == N - i
       {
-        arr[i+1] := arr[i]; // shift right
+        arr[i+1] := arr[i];              // shift right
         assert arr[i+1] == old(arr[i]);
-        t := t + 1.0;
+        c.Inc(); //t := t + 1.0;
       }
       assert arr[..k] == old(arr[..k]) == elems[..k];          // [0, k) is unchanged
       assert arr[k+1..N+1] == old(arr[k..N]) == elems[k+1..];  // [k, N] is right shifted 
 
       // 2. Insert x at position k
       arr[k] := x;
-      t := t + 1.0;
-
+      c.Inc();  //t := t + 1.0;
+     
       // Update number of elements
       nElems := nElems + 1;
       assert forall j :: 0 <= j < |elems| ==> arr[j] == elems[j];
 
-      assert t == (N - k + 1) as R0 == Tinsert(N, k) 
-               <= (N + 1) as R0     == Tinsert2(N);
-      assert Tinsert2 in O(linGrowth()) by { var c, n0 := lem_Insert_Tinsert2BigOlin(); }      
-    }
-                                              
-    // Appends element x in the list
-    method Append(x:T) returns (ghost t:R0)
+      assert c.Count() == N - k + 1 == InsertCost<T>.Cost(c.Size(), k); 
+    }   
+
+    method Append_CostTest(x:T) returns (ghost c:Cost<AppendIn<T>>)  
       modifies this, Repr()    
       // Pre:
       requires Valid()
@@ -168,31 +166,117 @@ module ArrayList refines List {
       ensures  forall j :: 0 <= j < old(Size()) ==> Get(j).0 == old(Get(j).0)    // [0, old(Size())) is unchanged  
       ensures  Get(old(Size())).0 == x  
       // Complexity:
-      ensures  var N := old(Size()); && t == Tappend(N) 
-                                     && tIsBigO(N, t as R0, constGrowth())      
+      ensures  var N := old(Size()); c.Count() == AppendCost<T>.Cost(N)    
+    { 
+      var N := Size(); 
+      c := new AppendCost(arr, N, x); 
+      var c' := Insert_CostTest(N, x);
+      c.t := c'.t;
+      assert c.Count() == InsertCost<T>.Cost(N, N) == 1;     
+    }    
+
+    method OK_CostTest() returns (ghost c:Cost<OkIn<T>>)  
+      modifies this, Repr()     
+      // Pre:
+      requires Valid()
+      // Post:
+      ensures  Valid()     
+      ensures  tIsBigO(c.Size(), c.Count() as R0, linGrowth())   
     {
-      var N := Size();
-      t := Insert(N, x);
-      assert t == Tinsert(N, N) == 1 as R0; 
-      assert Tappend in O(constGrowth()) by { var c, n0 := lem_Append_TappendBigOconst(); }      
+      var N := Size(); 
+      c := new OkCost(arr, N); 
+      
+      c.t := 2*N;  
+
+      assert c.Count() == 2*N <= 2*arr.Length == OkCost<T>.Cost(arr.Length);
+      assert (n => OkCost<T>.Cost(n) as R0) in O(linGrowth()) 
+        by { var c, n0 := lem_OK_BigOlin<T>(); }      
     }
 
-    // Deletes element at position k in the list
-    method {:axiom} Delete(k:nat) returns (ghost t:R0)
-      modifies this, Repr()
-      // Pre:    
-      requires Valid()
-      requires 0 <= k < Size()
-      // Post:
-      ensures  Valid() && fresh(Repr() - old(Repr()))
-      ensures  Size() == old(Size()) - 1
-      ensures  forall j :: 0 <= j < k      ==> Get(j).0 == old(Get(j).0)
-      ensures  forall j :: k <= j < Size() ==> Get(j).0 == old(Get(j+1).0)   
-      // Complexity:
-      ensures  var N := old(Size()); && t <= Tdelete(N)
-                                     && tIsBigO(N, t as R0, linGrowth())       
-      // TODO: implementation with array shift here
+  }
+
+  /***********************************************/
+
+  class {:ghost} InsertCost<T> extends Cost<InsertIn<T>> {
+    ghost constructor(arr:array<T>, nElems:nat, k:nat, x_:T) 
+      requires k <= nElems
+      ensures Count() == 0
+      ensures Input() == (arr, nElems, k, x_) 
+    {
+      t, x := 0, (arr, nElems, k, x_);
+    }
+   
+    ghost function Size(): nat
+      reads this
+    { 
+      x.1 
+    }
+
+    ghost static function Cost(N:nat, k:nat) : nat
+      requires N >= k
+    {
+      N - k + 1
+    }
 
   }
+
+  class {:ghost} AppendCost<T> extends Cost<AppendIn<T>> {
+    ghost constructor(arr:array<T>, nElems:nat, x_:T)
+      ensures Count() == 0
+      ensures Input() == (arr, nElems, x_) 
+    {
+      t, x := 0, (arr, nElems, x_);
+    }
+  
+    ghost function Size(): nat
+      reads this
+    { 
+      x.1 
+    }
+
+    ghost static function Cost(N:nat) : nat
+    {
+      1
+    }
+  }
+
+  class {:ghost} OkCost<T> extends Cost<OkIn<T>> {
+    ghost constructor(arr:array<T>, nElems:nat)
+      ensures Count() == 0
+      ensures Input() == (arr, nElems) 
+    {
+      t, x := 0, (arr, nElems);
+    }
+  
+    ghost function Size(): nat
+      reads this
+    { 
+      x.0.Length 
+    }
+
+    ghost static function Cost(N:nat) : nat
+    {
+      2*N
+    }
+  }
+
+  lemma lem_OK_BigOlin<T>() returns (c:R0, n0:nat) 
+    ensures c > 0.0 && bigOfrom(c, n0, (n => OkCost<T>.Cost(n) as R0), linGrowth())
+  {
+    c, n0 := 2.0, 1;
+    forall n:nat | 0 <= n0 <= n
+      ensures (n => OkCost<T>.Cost(n) as R0)(n) <= c*linGrowth()(n)
+    {
+      calc {
+           (n => OkCost<T>.Cost(n) as R0)(n);
+        == (2*n)  as R0;
+        <= c*n as R0;
+        == { lem_expOne(n as R0); }
+           c*exp(n as R0, 1.0);
+        == c*linGrowth()(n);   
+      }
+    }
+    assert bigOfrom(c, n0, (n => OkCost<T>.Cost(n) as R0), linGrowth());
+  }    
 
 }
