caseStudy/ADT/costAware/Cost2.dfy
@@ -1,0 +1,35 @@
+/******************************************************************************
+  Abstract Cost type
+******************************************************************************/
+
+module Cost2 {
+
+  trait {:ghost} {:termination false} Cost2<OpType, State> {
+    ghost var ops: seq<OpType>
+    ghost var totalCost: nat
+
+    ghost method Log(op:OpType, weight:nat := 1)
+      modifies this
+      ensures ops == old(ops) + [op]
+      ensures totalCost == old(totalCost) + weight
+    {
+      ops := ops + [op];
+      totalCost := totalCost + weight;
+    }
+
+    ghost function Count(): nat
+      reads this
+    {
+      totalCost
+    }
+
+    ghost predicate OpsValid(init:State)
+      reads this
+
+    // Abstract: replay the operations on the initial state
+    ghost function ApplyOps(init:State): State
+      reads this
+      requires OpsValid(init)
+  }
+
+}
