caseStudy/ADT/costAware/Cost2ArrayList.dfy
@@ -1,0 +1,96 @@
+include "../../../theory/math/ExpReal.dfy"
+include "../../../theory/math/TypeR0.dfy"
+include "../../../theory/ComplexityR0.dfy"
+include "./Cost2List.dfy"
+
+/******************************************************************************
+  ArrayList ADT
+******************************************************************************/
+
+module Cost2ArrayList refines Cost2List {
+
+  datatype ArrayOp<T> = Write(i: nat, v: T)  // | Shift(from: nat, to: nat)
+
+  type State<T> = seq<T>
+
+  trait Cost2ArrayList<T(0)> extends Cost2List<T, ArrayOp<T>, State<T>> { 
+
+    ghost var elems:seq<T>  // ghost model for physical array arr
+
+    /******************************************************************************
+      Query operations
+    ******************************************************************************/
+
+    // Returns true iff the model is consistent with the data
+    ghost predicate ValidModel()
+      reads this, Repr()
+      requires Valid()      
+    {
+      && Size() == |elems| 
+      && (forall i :: 0 <= i < Size() ==> Get(i).0 == elems[i])
+    }    
+    
+    /******************************************************************************
+      Update operations
+    ******************************************************************************/
+    
+    //Experiment with cost objects
+
+    // Inserts element x at position k in the list
+    method Insert(k:nat, x:T) returns (ghost c:Cost2<ArrayOp<T>, State<T>>)
+      modifies this, Repr()  
+      // Pre:
+      requires Valid() && ValidModel()
+      requires 0 <= k <= Size()
+      requires !IsFull()
+      // Post:
+      ensures  Valid() && ValidModel() && fresh(Repr() - old(Repr()))
+      ensures  Size() == old(Size()) + 1
+      ensures  forall j :: 0 <= j < k           ==> Get(j).0 == old(Get(j).0)    // [0, k)           is unchanged  
+      ensures  forall j :: k < j <= old(Size()) ==> Get(j).0 == old(Get(j-1).0)  // [k, old(Size())) is right shifted 
+      ensures  Get(k).0 == x                                                     // xs[k] == x
+      // Cost:
+      ensures  c.OpsValid(old(elems))            
+      ensures  c.ApplyOps(old(elems)) == elems    // Even this does not prevent under-reporting of cost.
+      ensures  c.Count() == old(Size()) - k + 1
+
+    method Append(x:T) returns (ghost c:Cost2<ArrayOp<T>, State<T>>)  
+      modifies this, Repr()    
+      // Pre:
+      requires Valid() && ValidModel()
+      requires !IsFull()
+      // Post:
+      ensures  Valid() && ValidModel()
+      ensures  Size() == old(Size()) + 1
+      ensures  forall j :: 0 <= j < old(Size()) ==> Get(j).0 == old(Get(j).0)    // [0, old(Size())) is unchanged  
+      ensures  Get(old(Size())).0 == x  
+
+  }
+
+  /***********************************************/
+
+  class {:ghost} ArrayInsertCost<T> extends Cost2<ArrayOp<T>, seq<T>> {
+
+    ghost constructor()
+      ensures ops == []
+    { 
+      ops := []; 
+      totalCost := 0;
+    }
+
+    ghost predicate OpsValid(init:seq<T>)
+      reads this
+    {
+      true // TODO
+    }
+
+    ghost function ApplyOps(init:seq<T>): seq<T>
+      reads this
+      requires OpsValid(init)
+    {
+      init  // TODO
+    }
+
+  }
+
+}
