caseStudy/ADT/costAware/Cost2ArrayListImpl.dfy
@@ -1,28 +1,20 @@
-include "../../../../theory/math/ExpReal.dfy"
-include "../../../../theory/math/TypeR0.dfy"
-include "../../../../theory/ComplexityR0.dfy"
-include "../List.dfy"
-include "./LemArrayList.dfy"
+include "../../../theory/math/ExpReal.dfy"
+include "../../../theory/math/TypeR0.dfy"
+include "../../../theory/ComplexityR0.dfy"
+include "./Cost2ArrayList.dfy"
+//include "./LemArrayList.dfy"
 //include "./CostArrayList.dfy"
 
 /******************************************************************************
-  Array implementation of a List
+  Implementation of ArrayList ADT
 ******************************************************************************/
 
-module ArrayList refines List {
+module Cost2ArrayListImpl refines Cost2ArrayList {
 
-  import opened LemArrayList
-  
-  // Refine input type for each relevant operation
-  type InsertIn<T> = (array<T>, nat, nat, T)    
-  type AppendIn<T> = (array<T>, nat, T)   
-  type OkIn<T> = (array<T>, nat)   
-
-  class ArrayList<T(0)> extends List<T> {
+  class Cost2ArrayListImpl<T(0)> extends Cost2ArrayList<T> {
 
     var arr:array<T>
     var nElems:nat
-    ghost var elems:seq<T>  // ghost model for physical array arr
 
     constructor(capacity:nat)
       // Pre:
@@ -32,17 +24,10 @@ module ArrayList refines List {
       ensures arr.Length == capacity
       ensures Size() == 0
     {
-      arr := new T[capacity];  
+      arr := new T[capacity];   
       nElems := 0; 
       elems := [];
     }   
-
-    // default constructor
-    static method Create<T(0)>() returns (obj:ArrayList)
-      ensures obj.arr.Length == 1
-    {
-      obj := new ArrayList<T>(1);
-    }
 
     /******************************************************************************
       Query operations
@@ -73,10 +58,10 @@ module ArrayList refines List {
       requires Valid()
       requires 0 <= i < Size() 
       // Complexity:
-      ensures var t := ret.1; t <= Tget(Size())
-      ensures var t := ret.1; tIsBigO(Size(), t as R0, constGrowth())      
+      //ensures var t := ret.1; t <= Tget(Size())
+      //ensures var t := ret.1; tIsBigO(Size(), t as R0, constGrowth())      
     {
-      lem_Get_TgetBigOconst();
+      //lem_Get_TgetBigOconst();
       (arr[i], ghost 1.0)
     }
 
@@ -95,103 +80,86 @@ module ArrayList refines List {
       && 0 < arr.Length
       && this in Repr() 
       && arr  in Repr()
-      // The array and its ghost counterpart are aligned
-      && nElems == |elems| 
-      && (forall i :: 0 <= i < nElems ==> arr[i] == elems[i])
     }    
 
     /******************************************************************************
       Update operations
     ******************************************************************************/
+    
+    //Experiment with cost objects
 
     // Inserts element x at position k in the list
-    method Insert(k:nat, x:T) returns (ghost t:R0)
-      modifies this, Repr()    
+    method Insert(k:nat, x:T) returns (ghost c:Cost2<ArrayOp<T>, State<T>>)
+      modifies this, Repr()  
       // Pre:
-      requires Valid()
+      requires Valid() && ValidModel()
       requires 0 <= k <= Size()
       requires !IsFull()
       // Post:
-      ensures  Valid() && fresh(Repr() - old(Repr()))
+      ensures  Valid() && ValidModel() && fresh(Repr() - old(Repr()))
       ensures  Size() == old(Size()) + 1
       ensures  forall j :: 0 <= j < k           ==> Get(j).0 == old(Get(j).0)    // [0, k)           is unchanged  
       ensures  forall j :: k < j <= old(Size()) ==> Get(j).0 == old(Get(j-1).0)  // [k, old(Size())) is right shifted 
       ensures  Get(k).0 == x                                                     // xs[k] == x
-      // Complexity:
-      ensures  var N := old(Size()); && t == Tinsert(N,k)
-                                     && tIsBigO(N, t as R0, linGrowth())                             
-    {
-      var N := Size();
-      t := 0.0;
+      // Cost:
+      ensures  c.OpsValid(old(elems))            
+      ensures  c.ApplyOps(old(elems)) == elems    // Even this does not prevent under-reporting of cost.
+      ensures  c.Count() == old(Size()) - k + 1
+    { 
+      c := new ArrayInsertCost(); assert c.Count() == 0;
+      var N := Size(); // == nElems 
 
       // Update model
+      assert nElems == |elems|; 
+      assert (forall i :: 0 <= i < nElems ==> arr[i] == elems[i]);
       elems := elems[..k] + [x] + elems[k..];
       
       // Update array:
       // 1. Shift [k, N) to the right
       for i := N downto k
-        modifies arr
+        modifies arr, c
         invariant N < arr.Length
         invariant arr[..i]      == old(arr[..i])   // [0, i) is unchanged  
         invariant arr[i+1..N+1] == old(arr[i..N])  // (i, N) is right shifted        
-        invariant t == (N - i) as R0    
+        invariant c.Count() == N - i
       {
-        arr[i+1] := arr[i]; // shift right
+        arr[i+1] := arr[i];              // shift right
         assert arr[i+1] == old(arr[i]);
-        t := t + 1.0;
+        c.Log(Write(i+1, arr[i]), 1); //t := t + 1.0;
       }
       assert arr[..k] == old(arr[..k]) == elems[..k];          // [0, k) is unchanged
       assert arr[k+1..N+1] == old(arr[k..N]) == elems[k+1..];  // [k, N] is right shifted 
 
       // 2. Insert x at position k
       arr[k] := x;
-      t := t + 1.0;
-
+      c.Log(Write(k, x), 1);  //t := t + 1.0;
+     
       // Update number of elements
       nElems := nElems + 1;
       assert forall j :: 0 <= j < |elems| ==> arr[j] == elems[j];
 
-      assert t == (N - k + 1) as R0 == Tinsert(N, k) 
-               <= (N + 1) as R0     == Tinsert2(N);
-      assert Tinsert2 in O(linGrowth()) by { var c, n0 := lem_Insert_Tinsert2BigOlin(); }      
-    }
-                                              
-    // Appends element x in the list
-    method Append(x:T) returns (ghost t:R0)
+      assert c.Count() == N - k + 1; 
+    }   
+
+    method Append(x:T) returns (ghost c:Cost2<ArrayOp<T>, State<T>>)  
       modifies this, Repr()    
       // Pre:
-      requires Valid()
+      requires Valid() && ValidModel()
       requires !IsFull()
       // Post:
-      ensures  Valid()
+      ensures  Valid() && ValidModel()
       ensures  Size() == old(Size()) + 1
       ensures  forall j :: 0 <= j < old(Size()) ==> Get(j).0 == old(Get(j).0)    // [0, old(Size())) is unchanged  
       ensures  Get(old(Size())).0 == x  
       // Complexity:
-      ensures  var N := old(Size()); && t == Tappend(N) 
-                                     && tIsBigO(N, t as R0, constGrowth())      
-    {
-      var N := Size();
-      t := Insert(N, x);
-      assert t == Tinsert(N, N) == 1 as R0; 
-      assert Tappend in O(constGrowth()) by { var c, n0 := lem_Append_TappendBigOconst(); }      
-    }
-
-    // Deletes element at position k in the list
-    method {:axiom} Delete(k:nat) returns (ghost t:R0)
-      modifies this, Repr()
-      // Pre:    
-      requires Valid()
-      requires 0 <= k < Size()
-      // Post:
-      ensures  Valid() && fresh(Repr() - old(Repr()))
-      ensures  Size() == old(Size()) - 1
-      ensures  forall j :: 0 <= j < k      ==> Get(j).0 == old(Get(j).0)
-      ensures  forall j :: k <= j < Size() ==> Get(j).0 == old(Get(j+1).0)   
-      // Complexity:
-      ensures  var N := old(Size()); && t <= Tdelete(N)
-                                     && tIsBigO(N, t as R0, linGrowth())       
-      // TODO: implementation with array shift here
+      //ensures  var N := old(Size()); c.Count() == AppendCost<T>.Cost(N)    
+  //  { 
+      // var N := Size(); 
+      // c := new AppendCost(arr, N, x); 
+      // var c' := Insert_CostTest(N, x);
+      // c.t := c'.t;
+      // assert c.Count() == InsertCost<T>.Cost(N, N) == 1;     
+   // }    
 
   }
 
